proof that the spectrum of a ring is a sheaf completed

Comm_Ring_Theory.thy
@@ -386,21 +386,7 @@ qed
 definition is_zariski_open:: "'a set set \<Rightarrow> bool"
   where "is_zariski_open U \<equiv> generated_topology {U. \<exists>\<aa>. ideal \<aa> R (+) (\<cdot>) \<zero> \<one> \<and> U = Spec - \<V> \<aa>} U"
 
-lemma is_zariski_open_empty [simp]: "is_zariski_open {}"
-  using UNIV is_zariski_open_def by blast
-
-lemma is_zariski_open_Spec [simp]: "is_zariski_open Spec"
-  by (simp add: UNIV is_zariski_open_def)
-
-lemma is_zariski_open_Union [intro]: 
-  "(\<And>x. x \<in> F \<Longrightarrow> is_zariski_open x) \<Longrightarrow> is_zariski_open (\<Union> F)"
-  by (simp add: UNIV is_zariski_open_def)
-
-lemma is_zariski_open_Int [simp]: 
-  "\<lbrakk>is_zariski_open U; is_zariski_open V\<rbrakk> \<Longrightarrow> is_zariski_open (U \<inter> V)"
-  by (simp add: Int is_zariski_open_def)
-
-lemma zarisky_is_topological_space [iff]:
+lemma zarisky_is_topological_space:
   shows "topological_space Spec is_zariski_open"
 proof qed (auto simp: is_zariski_open_def spectrum_def  UNIV)
 
@@ -697,7 +683,7 @@ next
   assume oc: "open_cover_of_open_subset X' is_open' U I V"
     and VU: "\<And>i. i \<in> I \<Longrightarrow> V i \<subseteq> U"
     and s: "s \<in> direct_im_sheaf U"
-    and eq0: "\<And>i. i \<in> I \<Longrightarrow> direct_im_sheaf_morphisms U (V i) s = \<zero>\<^bsub>f \<^sup>\<inverse> X (V i)\<^esub>"
+    and eq0: "\<And>i. (i::real) \<in> I \<Longrightarrow> direct_im_sheaf_morphisms U (V i) s = \<zero>\<^bsub>f \<^sup>\<inverse> X (V i)\<^esub>"
   have "open_cover_of_open_subset X is_open (f\<^sup>\<inverse> X U) I (\<lambda>i. f\<^sup>\<inverse> X (V i))"
     by (simp add: oc open_cover_of_open_subset_from_target_to_source) 
   then show "s = \<zero>\<^bsub>f \<^sup>\<inverse> X U\<^esub>"
@@ -1206,29 +1192,21 @@ lemma map_on_empty_is_regular:
   shows "is_regular s {}"
   by (simp add: is_regular_def)
 
-definition sheaf_on_spec:: "('a set) set \<Rightarrow> ('a set \<Rightarrow> ('a \<times> 'a) set) set" ("\<O> _" [900] 900)
+definition sheaf_on_spec:: "('a set) set \<Rightarrow> ('a set \<Rightarrow> ('a \<times> 'a) set) set" ("\<O> _")
   where "\<O> U \<equiv> {s. (Set_Theory.map s U (\<Union>\<pp>\<in>U. (R\<^bsub>\<pp> (+) (\<cdot>) \<zero>\<^esub>))) 
                   \<and> is_regular s U}"
 
 lemma sheaf_on_spec_of_empty_is_singleton:
   fixes U:: "'a set set"
-  assumes "U = {}" and "s \<in> {s. Set_Theory.map s U (\<Union>\<pp>\<in>U. (R\<^bsub>\<pp> (+) (\<cdot>) \<zero>\<^esub>))}" 
-      and "t \<in> {s. Set_Theory.map s U (\<Union>\<pp>\<in>U. (R\<^bsub>\<pp> (+) (\<cdot>) \<zero>\<^esub>))}"
+  assumes "U = {}" and "s \<in> {s. Set_Theory.map s U (\<Union>\<pp>\<in>U. (R\<^bsub>\<pp> (+) (\<cdot>) \<zero>\<^esub>))}" and 
+"t \<in> {s. Set_Theory.map s U (\<Union>\<pp>\<in>U. (R\<^bsub>\<pp> (+) (\<cdot>) \<zero>\<^esub>))}"
   shows "s = t"
   using assms by (simp add: Set_Theory.map_def)
-
-lemma sheaf_on_spec_empty [simp]: "sheaf_on_spec {} = {\<lambda>\<pp>. undefined}"
-  proof
-    show "{\<lambda>\<pp>. undefined} \<subseteq> \<O> {}"
-      using undefined_is_map_on_empty map_on_empty_is_regular sheaf_on_spec_def by fastforce
-    thus "\<O> {} \<subseteq> {\<lambda>\<pp>. undefined}" 
-      using sheaf_on_spec_def sheaf_on_spec_of_empty_is_singleton by auto
-  qed
 
 definition add_sheaf_on_spec:: "('a set) set \<Rightarrow> ('a set \<Rightarrow> ('a \<times> 'a) set) \<Rightarrow> ('a set \<Rightarrow> ('a \<times> 'a) set) \<Rightarrow> ('a set \<Rightarrow> ('a \<times> 'a) set)"
   where "add_sheaf_on_spec U s s' \<equiv> \<lambda>\<pp>\<in>U. cxt_quotient_ring.add_rel (R \<setminus> \<pp>) R (+) (\<cdot>) \<zero> (s \<pp>) (s' \<pp>)"
 
-lemma is_regular_add_sheaf_on_spec:
+lemma
   assumes "is_zariski_open U" and "is_regular s U" and "is_regular s' U" 
   shows "is_regular (add_sheaf_on_spec U s s') U"
   sorry
@@ -1236,7 +1214,7 @@ lemma is_regular_add_sheaf_on_spec:
 definition mult_sheaf_on_spec:: "('a set) set \<Rightarrow> ('a set \<Rightarrow> ('a \<times> 'a) set) \<Rightarrow> ('a set \<Rightarrow> ('a \<times> 'a) set) \<Rightarrow> ('a set \<Rightarrow> ('a \<times> 'a) set)"
   where "mult_sheaf_on_spec U s s' \<equiv> \<lambda>\<pp>\<in>U. cxt_quotient_ring.mult_rel (R \<setminus> \<pp>) R (+) (\<cdot>) \<zero> (s \<pp>) (s' \<pp>)"
 
-lemma is_regular_mult_sheaf_on_spec:
+lemma
   assumes "is_zariski_open U" and "is_regular s U" and "is_regular s' U" 
   shows "is_regular (mult_sheaf_on_spec U s s') U" sorry
 
@@ -1245,17 +1223,16 @@ definition zero_sheaf_on_spec:: "'a set set \<Rightarrow> ('a set \<Rightarrow> 
 
 lemma is_regular_zero_sheaf_on_spec:
   assumes "is_zariski_open U"
-  shows "is_regular (zero_sheaf_on_spec U) U"
-  sorry
+  shows "is_regular (zero_sheaf_on_spec U) U" sorry
 
 definition one_sheaf_on_spec:: "'a set set \<Rightarrow> ('a set \<Rightarrow> ('a \<times> 'a) set)"
   where "one_sheaf_on_spec U \<equiv> \<lambda>\<pp>\<in>U. cxt_quotient_ring.frac (R \<setminus> \<pp>) R (+) (\<cdot>) \<zero> \<one> \<one>"
 
-lemma is_regular_one_sheaf_on_spec:
+lemma 
   assumes "is_zariski_open U"
   shows "is_regular (one_sheaf_on_spec U) U" sorry
 
-lemma ring_sheaf_on_spec:
+lemma 
   assumes "is_zariski_open U"
   shows "ring (\<O> U) (add_sheaf_on_spec U) (mult_sheaf_on_spec U) (zero_sheaf_on_spec U) (one_sheaf_on_spec U)"
   sorry
@@ -1285,19 +1262,27 @@ lemma sheaf_on_spec_morphisms_are_ring_morphisms:
 lemma sheaf_on_spec_is_presheaf:
   shows "presheaf_of_rings Spec is_zariski_open sheaf_on_spec sheaf_on_spec_morphisms (\<lambda>\<pp>. undefined)
 (\<lambda>U. add_sheaf_on_spec U) (\<lambda>U. mult_sheaf_on_spec U) (\<lambda>U. zero_sheaf_on_spec U) (\<lambda>U. one_sheaf_on_spec U)"
-unfolding presheaf_of_rings_def presheaf_of_rings_axioms_def
-proof (intro conjI strip)
-  show "\<And>U. is_zariski_open U \<Longrightarrow> (\<And>s. s \<in> (\<O> U) \<Longrightarrow> sheaf_on_spec_morphisms U U s = s)"
+proof-
+  have "topological_space Spec is_zariski_open" by (simp add: zarisky_is_topological_space)
+  moreover have "sheaf_on_spec {} = {\<lambda>\<pp>. undefined}"
+  proof
+    show "{\<lambda>\<pp>. undefined} \<subseteq> \<O> {}"
+      using undefined_is_map_on_empty map_on_empty_is_regular sheaf_on_spec_def by fastforce
+    thus "\<O> {} \<subseteq> {\<lambda>\<pp>. undefined}" 
+      using sheaf_on_spec_def sheaf_on_spec_of_empty_is_singleton by auto
+  qed
+  moreover have "\<And>U. is_zariski_open U \<Longrightarrow> (\<And>s. s \<in> (\<O> U) \<Longrightarrow> sheaf_on_spec_morphisms U U s = s)"
     using sheaf_on_spec_morphisms_def sheaf_morphisms_on_sheaf_on_spec by simp
-  show "\<And>U V W. \<lbrakk>is_zariski_open U; is_zariski_open V; is_zariski_open W; V \<subseteq> U;
-                 W \<subseteq> V\<rbrakk> \<Longrightarrow> (\<And>s. s \<in> \<O> U \<Longrightarrow> sheaf_on_spec_morphisms U W s = (sheaf_on_spec_morphisms V W \<circ> sheaf_on_spec_morphisms U V) s)"
-      using restrict_further sheaf_on_spec_morphisms_are_maps map.map_closed
-    unfolding sheaf_on_spec_morphisms_def
-    by (smt (verit) FuncSet.restrict_restrict comp_apply inf.absorb_iff2 restrict_apply') 
-qed (auto simp: sheaf_on_spec_morphisms_are_ring_morphisms)
+  moreover have "\<And>U V W. is_zariski_open U \<Longrightarrow> is_zariski_open V \<Longrightarrow> is_zariski_open W \<Longrightarrow> V \<subseteq> U 
+\<Longrightarrow> W \<subseteq> V \<Longrightarrow> (\<And>s. s \<in> \<O> U \<Longrightarrow> sheaf_on_spec_morphisms U W s = (sheaf_on_spec_morphisms V W \<circ> sheaf_on_spec_morphisms U V) s)"
+    using sheaf_on_spec_morphisms_def restrict_further sheaf_on_spec_morphisms_are_maps map.map_closed
+  by (smt FuncSet.restrict_restrict inf.absorb_iff2 o_apply restrict_apply')
+  ultimately show ?thesis 
+    unfolding presheaf_of_rings_def presheaf_of_rings_axioms_def using sheaf_on_spec_morphisms_are_ring_morphisms by blast
+qed
 
 (* ex. 0.30 *)
-lemma
+lemma sheaf_on_spec_is_sheaf:
   shows "sheaf_of_rings Spec is_zariski_open sheaf_on_spec sheaf_on_spec_morphisms (\<lambda>\<pp>. undefined)
 (\<lambda>U. add_sheaf_on_spec U) (\<lambda>U. mult_sheaf_on_spec U) (\<lambda>U. zero_sheaf_on_spec U) (\<lambda>U. one_sheaf_on_spec U)"
 proof (intro sheaf_of_rings.intro sheaf_of_rings_axioms.intro)
@@ -1309,11 +1294,11 @@ next
                         "\<And>i. i \<in> I \<Longrightarrow> V i \<subseteq> U" 
                         "s \<in> \<O> U" 
                         "\<And>i. i \<in> I \<Longrightarrow> sheaf_on_spec_morphisms U (V i) s = zero_sheaf_on_spec (V i)"
-  then have "s \<pp> = zero_sheaf_on_spec U \<pp>" if "\<pp> \<in> U" for \<pp>
-  proof -
-    obtain i where F: "i \<in> I" "\<pp> \<in> (V i)" "is_zariski_open (V i)" 
-      using \<open>\<pp> \<in> U\<close> H(1) open_cover_of_subset.cover_of_select_index_is_open cover_of_subset.cover_of_select_index 
-        cover_of_subset.select_index_belongs open_cover_of_open_subset.axioms(1) open_cover_of_subset_def by fastforce
+  then have "\<And>\<pp>. \<pp> \<in> U \<Longrightarrow> s \<pp> = zero_sheaf_on_spec U \<pp>"
+  proof-
+    fix \<pp> assume "\<pp> \<in> U" then obtain i where F: "i \<in> I" "\<pp> \<in> (V i)" "is_zariski_open (V i)" 
+      using H(1) open_cover_of_subset.cover_of_select_index_is_open cover_of_subset.cover_of_select_index 
+cover_of_subset.select_index_belongs open_cover_of_open_subset.axioms(1) open_cover_of_subset_def by fastforce
     then have "sheaf_on_spec_morphisms U (V i) s \<pp> = cxt_quotient_ring.frac (R \<setminus> \<pp>) R (+) (\<cdot>) \<zero> \<zero> \<one>"  
       using H(2,4) F by (simp add: zero_sheaf_on_spec_def) 
     thus "s \<pp> = zero_sheaf_on_spec U \<pp>" 
@@ -1322,54 +1307,79 @@ next
   then show "s = zero_sheaf_on_spec U"
     by (metis (mono_tags, lifting) H(3) comm_ring.sheaf_on_spec_def comm_ring.zero_sheaf_on_spec_def local.comm_ring_axioms mem_Collect_eq restrict_apply' restrict_ext restrict_on_source)
 next
-  fix U I V s 
-  assume H: "open_cover_of_open_subset Spec is_zariski_open U I V"
-            "\<forall>i. i \<in> I \<longrightarrow> V i \<subseteq> U \<and> s i \<in> \<O> (V i)"
-            "\<And>i j. i \<in> I \<Longrightarrow>
-                      j \<in> I \<Longrightarrow>
-                        sheaf_on_spec_morphisms (V i) (V i \<inter> V j) (s i) =
-                        sheaf_on_spec_morphisms (V j) (V i \<inter> V j) (s j)"
+  fix U I V s assume H: "open_cover_of_open_subset Spec is_zariski_open U I V"
+                        "\<forall>i. i \<in> I \<longrightarrow> V i \<subseteq> U \<and> s i \<in> \<O> (V i)"
+                        "\<And>i j. i \<in> I \<Longrightarrow>
+                                  j \<in> I \<Longrightarrow>
+                                    sheaf_on_spec_morphisms (V i) (V i \<inter> V j) (s i) =
+                                    sheaf_on_spec_morphisms (V j) (V i \<inter> V j) (s j)"
   define t where D: "t \<equiv> \<lambda>\<pp>\<in>U. s (cover_of_subset.select_index I V \<pp>) \<pp>"
-  then have F1: "s i \<pp> = s j \<pp>" if "i \<in> I" "j \<in> I" "\<pp> \<in> V i" "\<pp> \<in> V j" for \<pp> i j
+  then have F1: "\<And>\<pp> i j. i \<in> I \<Longrightarrow> j \<in> I \<Longrightarrow> \<pp> \<in> V i \<Longrightarrow> \<pp> \<in> V j \<Longrightarrow> s i \<pp> = s j \<pp>"
   proof-
-    have "s i \<pp> = sheaf_on_spec_morphisms (V i) (V i \<inter> V j) (s i) \<pp>"
-      using that sheaf_on_spec_morphisms_def by (simp add: H(2))
+    fix \<pp> i j assume h: "i \<in> I" "j \<in> I" "\<pp> \<in> V i" "\<pp> \<in> V j"
+    then have "s i \<pp> = sheaf_on_spec_morphisms (V i) (V i \<inter> V j) (s i) \<pp>"
+      using sheaf_on_spec_morphisms_def by (simp add: H(2))
     moreover have "\<dots> = sheaf_on_spec_morphisms (V j) (V i \<inter> V j) (s j) \<pp>"
-      using H(3) that by fastforce
+      using H(3) h(1,2) by fastforce
     moreover have "\<dots> = s j \<pp>" 
-      using sheaf_on_spec_morphisms_def that by (simp add: H(2))
+      using sheaf_on_spec_morphisms_def h(2) by (simp add: H(2) h(3,4))
     ultimately show "s i \<pp> = s j \<pp>" by blast
   qed
   moreover have "t \<in> \<O> U"
   proof-
     have "Set_Theory.map t U (\<Union>\<pp>\<in>U. (R\<^bsub>\<pp> (+) (\<cdot>) \<zero>\<^esub>))"
       by (metis UNIV insert_iff is_regular_def is_regular_zero_sheaf_on_spec is_zariski_open_def)
-    moreover have "is_regular t U" (* using D H(2) *)
-      unfolding is_regular_def
-    proof (intro strip conjI)
-      fix \<pp>
-      assume "\<pp> \<in> U" 
-      show "t \<pp> \<in> (R\<^bsub>\<pp> (+) (\<cdot>) \<zero>\<^esub>)"
-      proof -
-        obtain i where "i \<in> I \<and> \<pp> \<in> V i \<and> t \<pp> = (s i) \<pp>" 
+    moreover have "is_regular t U"
+    proof-
+      have "\<And>\<pp>. \<pp> \<in> U \<Longrightarrow> t \<pp> \<in> (R\<^bsub>\<pp> (+) (\<cdot>) \<zero>\<^esub>)" 
+      proof-
+        fix \<pp> assume "\<pp> \<in> U"
+        then obtain i where "i \<in> I \<and> \<pp> \<in> V i \<and> t \<pp> = (s i) \<pp>" 
           using cover_of_subset.select_index_belongs cover_of_subset.cover_of_select_index open_cover_of_open_subset.axioms(1) 
-            open_cover_of_subset_def D H(1) \<open>\<pp> \<in> U\<close> by fastforce 
+open_cover_of_subset_def D H(1) by fastforce 
         thus "t \<pp> \<in> (R\<^bsub>\<pp> (+) (\<cdot>) \<zero>\<^esub>)" using H(2) sheaf_on_spec_def is_regular_def by simp
       qed
-      show "\<exists>V. V \<subseteq> U \<and> \<pp> \<in> V \<and> (\<exists>r f. r \<in> R \<and> f \<in> R \<and> 
-               (\<forall>\<qq>. \<qq> \<in> V \<longrightarrow> f \<notin> \<qq>  \<and> t \<qq> = cxt_quotient_ring.frac (R \<setminus> \<qq>) R (+) (\<cdot>) \<zero> r f ))"
-        sorry
+      moreover have "(\<And>\<pp>. \<pp> \<in> U \<Longrightarrow> 
+              (\<exists>V. V \<subseteq> U \<and> \<pp> \<in> V \<and> (\<exists>r f. r \<in> R \<and> f \<in> R \<and> (\<forall>\<qq>. \<qq> \<in> V \<longrightarrow> 
+                                                                        f \<notin> \<qq> 
+                                                                          \<and> 
+                                                                        t \<qq> = cxt_quotient_ring.frac (R \<setminus> \<qq>) R (+) (\<cdot>) \<zero> r f
+))))"
+      proof-
+        fix \<pp> assume "\<pp> \<in> U"
+        then have "\<exists>V'. V'\<subseteq>V (cover_of_subset.select_index I V \<pp>) \<and> \<pp> \<in> V' \<and>
+                 (\<exists>r f. r \<in> R \<and>
+                        f \<in> R \<and>
+                        (\<forall>\<qq>. \<qq> \<in> V' \<longrightarrow>
+                             f \<notin> \<qq> \<and> s (cover_of_subset.select_index I V \<pp>) \<qq> = cxt_quotient_ring.frac (R\<setminus>\<qq>) R (+) (\<cdot>) \<zero> r f))"
+          using H(1,2) cover_of_subset.cover_of_select_index cover_of_subset.select_index_belongs is_regular_def mem_Collect_eq open_cover_of_open_subset_def open_cover_of_subset_def sheaf_on_spec_def by fastforce
+        moreover have "V (cover_of_subset.select_index I V \<pp>) \<subseteq> U" 
+          using H(2) by (meson H(1) \<open>\<pp> \<in> U\<close> cover_of_subset.select_index_belongs open_cover_of_open_subset_def open_cover_of_subset_def)
+        ultimately show "\<exists>V. V \<subseteq> U \<and> \<pp> \<in> V \<and> (\<exists>r f. r \<in> R \<and> f \<in> R \<and> (\<forall>\<qq>. \<qq> \<in> V \<longrightarrow> 
+                                                                        f \<notin> \<qq> 
+                                                                          \<and> 
+                                                                        t \<qq> = cxt_quotient_ring.frac (R \<setminus> \<qq>) R (+) (\<cdot>) \<zero> r f))"
+        proof-
+          have "\<And>V' \<qq>. V' \<subseteq> V (cover_of_subset.select_index I V \<pp>) \<Longrightarrow> \<qq> \<in> V' \<Longrightarrow> t \<qq> = s (cover_of_subset.select_index I V \<pp>) \<qq>"
+            using D F1 cover_of_subset.select_index_belongs
+            by (smt H(1) \<open>V (cover_of_subset.select_index I V \<pp>) \<subseteq> U\<close> \<open>\<pp> \<in> U\<close> cover_of_subset.cover_of_select_index in_mono open_cover_of_open_subset.axioms(1) open_cover_of_subset_def restrict_apply)
+          thus ?thesis
+            by (smt \<open>V (cover_of_subset.select_index I V \<pp>) \<subseteq> U\<close> \<open>\<exists>V'\<subseteq>V (cover_of_subset.select_index I V \<pp>). \<pp> \<in> V' \<and> (\<exists>r f. r \<in> R \<and> f \<in> R \<and> (\<forall>\<qq>. \<qq> \<in> V' \<longrightarrow> f \<notin> \<qq> \<and> s (cover_of_subset.select_index I V \<pp>) \<qq> = cxt_quotient_ring.frac (R\<setminus>\<qq>) R (+) (\<cdot>) \<zero> r f))\<close> subset_trans)
+        qed 
+      qed
+      ultimately show ?thesis using is_regular_def by simp
     qed
     ultimately show ?thesis using sheaf_on_spec_def by simp
   qed
-  have "sheaf_on_spec_morphisms U (V i) t = s i" if "i \<in> I" for i
+  have "\<And>i. i \<in> I \<Longrightarrow> sheaf_on_spec_morphisms U (V i) t = s i"
   proof
-    fix \<pp>
-    have "sheaf_on_spec_morphisms U (V i) t \<pp> = s i \<pp>" if "\<pp> \<in> U"
+    fix i \<pp> assume "i \<in> I"
+    have "\<pp> \<in> U \<Longrightarrow> sheaf_on_spec_morphisms U (V i) t \<pp> = s i \<pp>"
     proof-
-      obtain j where "j \<in> I \<and> \<pp> \<in> V j \<and> t \<pp> = s j \<pp>" 
+      assume "\<pp> \<in> U" 
+      then obtain j where "j \<in> I \<and> \<pp> \<in> V j \<and> t \<pp> = s j \<pp>" 
         using cover_of_subset.select_index_belongs cover_of_subset.cover_of_select_index open_cover_of_open_subset.axioms(1) 
-open_cover_of_subset_def D H(1) \<open>\<pp> \<in> U\<close> by fastforce
+open_cover_of_subset_def D H(1) by fastforce
       thus "sheaf_on_spec_morphisms U (V i) t \<pp> = s i \<pp>" 
         using sheaf_on_spec_morphisms_def D F1 
         by (smt H(2) \<open>i \<in> I\<close> \<open>t \<in> \<O> U\<close> mem_Collect_eq restrict_apply restrict_on_source sheaf_on_spec_def)
